theories/zoo_parabs/vertex__types.v
@@ -2,7 +2,7 @@ Require Import zoo.prelude.
 Require Import zoo.language.typeclasses.
 Require Import zoo.language.notations.
 Require Export zoo_parabs.pool.
-Require Export zoo_saturn.mpmc_stack_2.
+Require Export zoo_saturn.stack_mpmc_2.
 Require Export zoo_std.clist.
 Require Import zoo.options.
 
