theories/zoo_saturn/mpmc_stack_2__opaque.v
@@ -1,7 +1,0 @@
-Require Import zoo_saturn.mpmc_stack_2__code.
-
-#[global] Opaque mpmc_stack_2٠create.
-#[global] Opaque mpmc_stack_2٠push.
-#[global] Opaque mpmc_stack_2٠pop.
-#[global] Opaque mpmc_stack_2٠is_closed.
-#[global] Opaque mpmc_stack_2٠close.
