theories/zoo_saturn/stack_mpmc_2__opaque.v
@@ -1,0 +1,7 @@
+Require Import zoo_saturn.stack_mpmc_2__code.
+
+#[global] Opaque stack_mpmc_2٠create.
+#[global] Opaque stack_mpmc_2٠push.
+#[global] Opaque stack_mpmc_2٠pop.
+#[global] Opaque stack_mpmc_2٠is_closed.
+#[global] Opaque stack_mpmc_2٠close.
